with Tahina, writing pairs

src/lowparse/TestPair.fst
@@ -32,13 +32,13 @@ let read_components (i:irepr P.pair_parser)
     x, y
 
 module B = LowStar.Buffer
-assume val frozen_until (f:FB.fbuffer)
-  : Stack UInt32.t
-    (requires fun h ->
-      FB.recallable f \/ B.live h f)
-    (ensures fun h0 x h1 ->
-      h0 == h1 /\
-      FB.get_w (B.as_seq h0 f) == UInt32.v x)
+// assume val frozen_until (f:FB.fbuffer)
+//   : Stack UInt32.t
+//     (requires fun h ->
+//       FB.recallable f \/ B.live h f)
+//     (ensures fun h0 x h1 ->
+//       h0 == h1 /\
+//       FB.get_w (B.as_seq h0 f) == UInt32.v x)
 
 let read_components2 (i:irepr P.pair_parser)
   : Stack (x: (irepr LPI.parse_u32 * irepr LPI.parse_u16) { LM.irepr_v i == {P.fst = LM.irepr_v (fst x); P.snd = LM.irepr_v (snd x)} } )
@@ -70,3 +70,88 @@ let read_components3 (i:irepr P.pair_parser)
   havoc();
   let xsnd = LM.iaccess P.accessor_pair_snd i in
   (xfst, xsnd)
+
+module HS = FStar.HyperStack
+let frozen_until (h:HS.mem) : GTot nat =
+  FB.get_w (B.as_seq h buf.base)
+module U32 = FStar.UInt32
+
+module LMI = LowParse.MLow.Int
+
+let iwrite_u16 (u:UInt16.t) (p:UInt32.t)
+  : Stack (irepr LPI.parse_u16)
+    (requires fun h ->
+      frozen_until h <= U32.v p /\
+      U32.v p + 2 < U32.v buf.len)
+    (ensures fun h0 i h1 ->
+      LM.irepr_pos i == p /\
+      LM.irepr_pos' i == U32.(p +^ 2ul) /\
+      LM.irepr_v i == u   /\
+      frozen_until h1 == U32.v p + 2 /\
+      B.modifies (B.loc_buffer buf.base) h0 h1)
+   = FB.recall_w_default buf.base;
+     B.recall buf.base;
+     let h0 = get () in
+     let p' = LMI.write_u16 u buf p in
+     LM.loc_slice_from_to_eq buf 0ul 4ul;
+     let h1 = get () in
+     let p' = p `U32.add` 2ul in
+     B.modifies_buffer_from_to_elim buf.base 0ul 4ul (LM.loc_slice_from_to buf p p') h0 h1;
+     FB.recall_w_default buf.base;
+     FB.freeze buf.base p' ;
+     let h2 = get () in
+     LM.valid_exact_ext_intro LPI.parse_u16 h1 buf p p' h2 buf p p' ;
+     LM.witness_valid buf p
+
+
+let iwrite_u32 (u:UInt32.t) (p:UInt32.t)
+  : Stack (irepr LPI.parse_u32)
+    (requires fun h ->
+      frozen_until h <= U32.v p /\
+      U32.v p + 4 < U32.v buf.len)
+    (ensures fun h0 i h1 ->
+      LM.irepr_pos i == p /\
+      LM.irepr_pos' i == U32.(p +^ 4ul) /\
+      LM.irepr_v i == u   /\
+      frozen_until h1 == U32.v p + 4 /\
+      B.modifies (B.loc_buffer buf.base) h0 h1)
+   = FB.recall_w_default buf.base;
+     B.recall buf.base;
+     let h0 = get () in
+     let p' = LMI.write_u32 u buf p in
+     LM.loc_slice_from_to_eq buf 0ul 4ul;
+     let h1 = get () in
+     let p' = p `U32.add` 4ul in
+     B.modifies_buffer_from_to_elim buf.base 0ul 4ul (LM.loc_slice_from_to buf p p') h0 h1;
+     FB.recall_w_default buf.base;
+     FB.freeze buf.base p' ;
+     let h2 = get () in
+     LM.valid_exact_ext_intro LPI.parse_u32 h1 buf p p' h2 buf p p' ;
+     LM.witness_valid buf p
+
+assume val havoc_l :
+  l:B.loc -> Stack unit (fun h -> True) (fun h0 _ h1 ->
+  B.modifies l h0 h1 /\
+  frozen_until h0 == frozen_until h1)
+
+assume val some_loc: B.loc
+
+let iwrite_pair (u0:UInt32.t) (u1:UInt16.t) (p:UInt32.t)
+  : Stack (irepr P.pair_parser)
+    (requires fun h ->
+      frozen_until h <= U32.v p /\
+      U32.v p + 6 < U32.v buf.len)
+    (ensures fun h0 i h1 ->
+      LM.irepr_pos i == p /\
+      LM.irepr_pos' i == U32.(p +^ 6ul) /\
+      LM.irepr_v i == P.({fst=u0; snd=u1})  /\
+      frozen_until h1 == U32.v p + 6 /\
+      B.modifies (B.loc_union some_loc (B.loc_buffer buf.base)) h0 h1)
+   = let i0 = iwrite_u32 u0 p in
+     havoc_l some_loc;
+     let i1 = iwrite_u16 u1 U32.(p +^ 4ul) in
+     let h = get () in
+     LM.recall_valid i0;
+     LM.recall_valid i1;
+     Pair.pair_valid h buf p;
+     LM.witness_valid buf p
